Modified the oracle contract so it won't use the Some projection.

Oracle2/Oracle2.fst
@@ -13,39 +13,59 @@ module TX = Zen.TxSkeleton
 module W = Zen.Wallet
 
 type args =
-    { commit: hash;
-      timestamp : timestamp;
-      oraclePubKey: option publicKey }
+    { commit       : hash
+    ; timestamp    : timestamp
+    ; oraclePubKey : publicKey
+    }
 
 type assets =
-    { commitment: asset;
-      attestation: asset }
+    { commitment  : asset
+    ; attestation : asset
+    }
 
 // compressed public key
 type cpk = byte ** hash
 
-let parseArgs (msg: option data): result args `cost` 235 = // 41
+let parseArgs (pk : option publicKey) (msg: option data): result args `cost` 267 = // 73
     let open OT in
     match msg with
     | Some (Collection (Dict dict)) -> begin
         let! commit = Dict.tryFind "Commit" dict in // 64
         let! timestamp = Dict.tryFind "Timestamp" dict in // 64
-        let! oraclePubKey = Dict.tryFind "OraclePubKey" dict // 64
-                            >>= Zen.Data.tryPublicKey in //2
-        match commit, timestamp with
-        | Some (Hash commit), Some (U64 timestamp) ->
+        let! oraclePubKey =
+          begin match pk with
+          | None ->
+              Dict.tryFind "OraclePubKey" dict // 64
+              >>= Zen.Data.tryPublicKey // 2
+          | Some pk ->
+              pk
+              |> incSome 66
+          end
+        in match commit, timestamp, oraclePubKey with
+        | Some (Hash commit), Some (U64 timestamp), Some oraclePubKey ->
             RT.ok ({ commit=commit;
                      timestamp=timestamp;
                      oraclePubKey=oraclePubKey })
-        | Some _, _ | None, _ ->
+        | _, Some (U64 _), Some _ ->
             RT.failw "Could not parse Commit"
-        | _, Some _ | _, None ->
+        | Some (Hash _), _, Some _ ->
             RT.failw "Could not parse Timestamp"
+        | Some (Hash _), Some (U64 _), None ->
+            RT.failw "Could not parse OraclePubKey"
+        | _, _, Some _ ->
+            RT.failw "Could not parse Commit & Timestamp"
+        | _, Some (U64 _), None ->
+            RT.failw "Could not parse Commit & OraclePubKey"
+        | Some (Hash _), _, None ->
+            RT.failw "Could not parse Timestamp & OraclePubKey"
+        | _, _, _ ->
+            RT.failw "Could not parse Timestamp, Timestamp, & OraclePubKey"
         end
     | _ -> RT.autoFailw "MessageBody must be a dictionary."
 
 // compress a public key
-let compress (pk:publicKey): cpk `cost` 305 = let open FStar.UInt8 in // 13
+let compress (pk:publicKey): cpk `cost` 305 =  // 13
+    let open FStar.UInt8 in
     let parity = (Zen.Array.item 32 pk %^ 2uy) +^ 2uy in
     let aux (i:nat{i < 32}): byte `cost` 5 =
         ret (Zen.Array.item (31-i) pk) in
@@ -61,16 +81,16 @@ let hashCPK (cpk:cpk): hash `cost` 227 = // 4
     updateCPK cpk Sha3.empty // 203
     >>= Sha3.finalize // 20
 
-let hashArgs (args:args{Some? args.oraclePubKey}): hash `cost` 786 = // 18
-    let! cpk = compress (Some?.v args.oraclePubKey) in // 305
+let hashArgs (args:args): hash `cost` 784 = // 16
+    let! cpk = compress args.oraclePubKey in
     Sha3.updateHash args.commit Sha3.empty // 192
     >>= Sha3.updateU64 args.timestamp // 48
     >>= updateCPK cpk // 203
     >>= Sha3.finalize // 20
 
-val mkAssets: contractId -> args:args{Some? args.oraclePubKey} -> assets `cost` 1016
+val mkAssets: contractId -> args:args -> assets `cost` 1014
 let mkAssets (v, h) args = // 18
-    let! argsHash = hashArgs args in // 786
+    let! argsHash = hashArgs args in // 784
     let! arsgHash2 = Sha3.updateHash argsHash Sha3.empty // 192
                      >>= Sha3.finalize in // 20
     ret ({ commitment=v,h,argsHash; attestation=v,h,arsgHash2 })
@@ -79,10 +99,9 @@ let mkAssets (v, h) args = // 18
 // Making a commitment
 //
 
-val commit: txSkeleton -> contractId -> publicKey -> args -> CR.t `cost` 1163
-let commit tx cid senderPK args = // 16
-    let args = { args with oraclePubKey=Some senderPK } in
-    let! ({commitment=commitment}) = mkAssets cid args in // 1016
+val commit: txSkeleton -> contractId -> publicKey -> args -> CR.t `cost` 1159
+let commit tx cid senderPK args = // 14
+    let! ({commitment=commitment}) = mkAssets cid args in // 1014
     // mint the commitment token
     TX.mint 1UL commitment tx // 64
     // lock the commitment token to the contract
@@ -110,50 +129,40 @@ let attestTx tx cid senderPK assets: txSkeleton `cost` 891 = // 27
     // lock the commitment token to the contract
     >>= TX.lockToContract assets.commitment 1UL cid // 64
 
-let attest' tx cid senderPK w (args:args) = // 22
-    match args.oraclePubKey with
-    | Some _ -> begin
-        let! assets = mkAssets cid args in // 1016
-        // the tx, minus contract wallet inputs
-        attestTx tx cid senderPK assets // 891
-        // add a commitment token from the contract wallet
-        >>= TX.fromWallet assets.commitment 1UL cid w // W.size w * 128 + 192
-        // return the tx
-        >>= CR.ofOptionTxSkel "Could not spend from wallet" // 3
-        end
-    | None ->
-        RT.autoFailw "Could not parse OraclePubKey"
-
-let attest: txSkeleton -> contractId -> publicKey -> w:wallet -> args
-            -> CR.t `cost` (W.size w * 128 + 2124) = attest'
+// (1014 + (891 + (Zen.Wallet.size w * 128 + 192) + 3) + 18)
+let attest tx cid senderPK w (args:args) : contractResult `cost` (2118 + W.size w * 128) = // 18
+    let! assets = mkAssets cid args in // 1014
+    // the tx, minus contract wallet inputs
+    attestTx tx cid senderPK assets // 891
+    // add a commitment token from the contract wallet
+    >>= TX.fromWallet assets.commitment 1UL cid w // W.size w * 128 + 192
+    // return the tx
+    >>= CR.ofOptionTxSkel "Could not spend from wallet" // 3
 
 //
 // Exports
 //
 
-val main: txSkeleton -> context -> contractId -> command: string
-          -> sender: sender -> option data -> w: wallet -> option data
-          -> CR.t `cost` begin match command, sender with
-                         | "Commit", PK _ -> 1418
-                         | "Attest", PK _ -> Zen.Wallet.size w * 128 + 2379
-                         | _ -> 20 end
-let main tx _ cid command sender msg w _ = // 20
+let main tx _ cid command sender msg w _ = // 21
+    let open RT in
     match command, sender with
     | "Commit", PK pk ->
-        parseArgs msg `RT.bind` commit tx cid pk // 235 + 1163
+        parseArgs (Some pk) msg // 267
+        >>= commit tx cid pk // 1159
         <: CR.t `cost` begin match command, sender with
-                       | "Commit", PK _ -> 1398
-                       | "Attest", PK _ -> Zen.Wallet.size w * 128 + 2359
+                       | "Commit", PK _ -> 267 + 1159
+                       | "Attest", PK _ -> 267 + 2118 + Zen.Wallet.size w * 128
                        | _ -> 0 end
     | "Attest", PK pk ->
-        parseArgs msg `RT.bind` attest tx cid pk w // 235 + (Zen.Wallet.size w * 128 + 2124)
+        parseArgs None msg // 267
+        >>= attest tx cid pk w // 2118 + W.size w * 128
     | _, PK pk ->
-        RT.failw "a"
+        failw "Command not recognized"
     | _, _ ->
-        RT.failw "b"
+        failw "Sender must be a public key"
 
-let cf _ _ command sender _ w _ : nat `cost` 15 = // 15
+let cf _ _ command sender _ w _ : nat `cost` 19 = // 19
     ret begin match command, sender with
-        | "Commit", PK _ -> 1418
-        | "Attest", PK _ -> Zen.Wallet.size w * 128 + 2379
-        | _ -> 20 end
+        | "Commit", PK _ -> 267 + 1159 + 21
+        | "Attest", PK _ -> 267 + 2118 + Zen.Wallet.size w * 128 + 21
+        | _ -> 21 <: nat end
